

## Exercise 7

### Case i) Poisson with canonical link

Suppose that  $y_i \sim \text{Poisson}(\mu_i)$ , with  $\log(\mu_i) = \beta_1 + \beta_2 x_i$ , in cui  $x_i \in \{0, 1\}$ .

The likelihood equations are:

$$\sum_{i=1}^m y_i = \sum_{i=1}^m \mu_i \quad \text{and} \quad \sum_{i=1}^m y_i x_i = \sum_{i=1}^m \mu_i x_i$$

where  $x_i = 1$ , with  $i = 1, \dots, m_A$ , so  $\sum_{i=1}^{m_A} y_i = \sum_{i=1}^{m_A} \mu_i$

However, note that  $\mu_i = \exp(\beta_1 + \beta_2 x_i)$ , therefore  $\mu_i = \mu_A = \exp(\beta_1 + \beta_2)$  for  $i = 1, \dots, m_A$ . Consequently

$$\frac{1}{m_A} \sum_{i=1}^{m_A} \mu_A = \frac{1}{m_A} \sum_{i=1}^{m_A} y_i \Rightarrow \hat{\mu}_i = \hat{\mu}_A = \bar{y}_A, \text{ for } i = 1, \dots, m_A.$$

Moreover

$$\sum_{i=1}^m y_i = \sum_{i=1}^m \mu_i \Leftrightarrow \sum_{i=m_A+1}^m y_i + \overbrace{\sum_{i=1}^{m_A} y_i}^{m_A \bar{y}_A} = \sum_{i=m_A+1}^m \mu_i + \overbrace{\sum_{i=1}^{m_A} \mu_i}^{m_A \bar{y}_A}$$

$$\Leftrightarrow \frac{1}{m_B} \sum_{i=m_A+1}^m y_i = \frac{1}{m_B} \sum_{i=m_A+1}^m \mu_i$$

with  $\mu_i = \exp(\beta_1 + \beta_2 \cdot 0) = \exp(\beta_1) = \mu_B$ ,  $i = m_A+1, \dots, m$ , from which we obtain that  $\hat{\mu}_B = \bar{y}_B$ .

## Case ii) Poisson with any link function

The likelihood equations in this case are

$$\sum_{i=1}^m \frac{y_i - \mu_i}{\mu_i} \cdot \frac{1}{g'(\mu_i)} = 0, \quad \text{and} \quad \sum_{i=1}^m \frac{y_i - \mu_i}{\mu_i} \cdot \frac{1}{g'(\mu_i)} x_i = 0.$$

where  $x_i \in \{0, 1\}$ , so that  $\mu_i = \mu_A = g^{-1}(\beta_1 + \beta_2)$  for  $i = 1, \dots, m_A$  and

$\mu_i = \mu_B = g^{-1}(\beta_1)$  for  $i = m_A + 1, \dots, m$ . Hence, the two equations become

$$\sum_{i=1}^{m_A} \frac{y_i - \mu_A}{\mu_A} \cdot \frac{1}{g'(\mu_A)} + \sum_{i=m_A+1}^m \frac{y_i - \mu_B}{\mu_B} \cdot \frac{1}{g'(\mu_B)} = 0, \quad \text{and} \quad \sum_{i=1}^{m_A} \frac{y_i - \mu_A}{\mu_A} \cdot \frac{1}{g'(\mu_A)} = 0$$

It implies that can be canceled.

Focusing on the second equation:

$$\sum_{i=1}^{m_A} \frac{y_i - \mu_A}{\mu_A} \cdot \frac{1}{g'(\mu_A)} = 0 \iff \sum_{i=1}^{m_A} y_i = \sum_{i=1}^{m_A} \mu_A \implies \hat{\mu}_A = \frac{1}{m_A} \sum_{i=1}^{m_A} y_i = \bar{y}_A$$

Similarly, from the first equation:

$$\sum_{i=m_A+1}^m \frac{y_i - \mu_B}{\mu_B} \cdot \frac{1}{g'(\mu_B)} = 0 \implies \sum_{i=m_A+1}^m y_i = \sum_{i=m_A+1}^m \mu_B \implies \hat{\mu}_B = \bar{y}_B.$$



### Case iii, general G2P

The proof is almost identical to case ii. The estimation equations are

$$\sum_{i=1}^m w_i \frac{(y_i - \mu_i)}{v(\mu_i)} \cdot \frac{1}{g(\mu_i)} = 0 \quad \text{and} \quad \sum_{i=1}^m w_i \frac{(y_i - \mu_i)}{v(\mu_i)} \cdot \frac{1}{g(\mu_i)} x_i = 0.$$

where  $x_i \in \{0, 1\}$ , so that  $\mu_i = \mu_A = g^{-1}(\beta_1 + \beta_2)$  for  $i = 1, \dots, m_A$  and

$\mu_i = \mu_B = g^{-1}(\beta_1)$  for  $i = m_A + 1, \dots, m$ . Hence, the two equations become

$$\sum_{i=1}^{m_A} w_i \frac{(y_i - \mu_A)}{v(\mu_A)} \cdot \frac{1}{g'(\mu_A)} + \sum_{i=m_A+1}^m w_i \frac{(y_i - \mu_B)}{v(\mu_B)} \cdot \frac{1}{g'(\mu_B)} = 0; \quad \sum_{i=1}^{m_A} w_i \frac{(y_i - \mu_A)}{v(\mu_A)} \cdot \frac{1}{g'(\mu_A)} = 0$$

It implies that can be cancelled

Focusing on the second equation:

$$\sum_{i=1}^{m_A} w_i \frac{(y_i - \mu_A)}{v(\mu_A)} \cdot \frac{1}{g'(\mu_A)} = 0 \iff \sum_{i=1}^{m_A} w_i y_i = \mu_A \sum_{i=1}^{m_A} w_i \implies \hat{\mu}_A = \frac{\sum_{i=1}^{m_A} w_i y_i}{\sum_{i=1}^{m_A} w_i} = \bar{y}_{w,A}$$

Similarly, you get from the first equation that

$$\sum_{i=m_A+1}^m w_i \frac{(y_i - \mu_B)}{v(\mu_B)} \cdot \frac{1}{g'(\mu_B)} = 0 \iff \sum_{i=m_A+1}^m w_i y_i = \mu_B \sum_{i=m_A+1}^m w_i \implies \hat{\mu}_B = \bar{y}_{w,B}$$